conversion of UNITY theories to new-style

src/HOL/UNITY/Constrains.thy
@@ -3,10 +3,10 @@
     Author:     Lawrence C Paulson, Cambridge University Computer Laboratory
     Copyright   1998  University of Cambridge
 
-Safety relations: restricted to the set of reachable states.
+Weak safety relations: restricted to the set of reachable states.
 *)
 
-Constrains = UNITY + 
+theory Constrains = UNITY:
 
 consts traces :: "['a set, ('a * 'a)set set] => ('a * 'a list) set"
 
@@ -14,35 +14,29 @@ consts traces :: "['a set, ('a * 'a)set set] => ('a * 'a list) set"
     Arguments MUST be curried in an inductive definition*)
 
 inductive "traces init acts"  
-  intrs 
+  intros 
          (*Initial trace is empty*)
-    Init  "s: init ==> (s,[]) : traces init acts"
+    Init:  "s: init ==> (s,[]) : traces init acts"
 
-    Acts  "[| act: acts;  (s,evs) : traces init acts;  (s,s'): act |]
-	   ==> (s', s#evs) : traces init acts"
+    Acts:  "[| act: acts;  (s,evs) : traces init acts;  (s,s'): act |]
+	    ==> (s', s#evs) : traces init acts"
 
 
 consts reachable :: "'a program => 'a set"
 
 inductive "reachable F"
-  intrs 
-    Init  "s: Init F ==> s : reachable F"
+  intros 
+    Init:  "s: Init F ==> s : reachable F"
 
-    Acts  "[| act: Acts F;  s : reachable F;  (s,s'): act |]
-	   ==> s' : reachable F"
-
-consts
-  Constrains :: "['a set, 'a set] => 'a program set"  (infixl "Co"     60)
-  op_Unless  :: "['a set, 'a set] => 'a program set"  (infixl "Unless" 60)
-
-defs
-  Constrains_def
-    "A Co B == {F. F : (reachable F Int A)  co  B}"
-
-  Unless_def
-    "A Unless B == (A-B) Co (A Un B)"
+    Acts:  "[| act: Acts F;  s : reachable F;  (s,s'): act |]
+	    ==> s' : reachable F"
 
 constdefs
+  Constrains :: "['a set, 'a set] => 'a program set"  (infixl "Co" 60)
+    "A Co B == {F. F : (reachable F Int A)  co  B}"
+
+  Unless  :: "['a set, 'a set] => 'a program set"     (infixl "Unless" 60)
+    "A Unless B == (A-B) Co (A Un B)"
 
   Stable     :: "'a set => 'a program set"
     "Stable A == A Co A"
@@ -54,5 +48,346 @@ constdefs
   (*Polymorphic in both states and the meaning of <= *)
   Increasing :: "['a => 'b::{order}] => 'a program set"
     "Increasing f == INT z. Stable {s. z <= f s}"
+
+
+(*** traces and reachable ***)
+
+lemma reachable_equiv_traces:
+     "reachable F = {s. EX evs. (s,evs): traces (Init F) (Acts F)}"
+apply safe
+apply (erule_tac [2] traces.induct)
+apply (erule reachable.induct)
+apply (blast intro: reachable.intros traces.intros)+
+done
+
+lemma Init_subset_reachable: "Init F <= reachable F"
+by (blast intro: reachable.intros)
+
+lemma stable_reachable [intro!,simp]:
+     "Acts G <= Acts F ==> G : stable (reachable F)"
+by (blast intro: stableI constrainsI reachable.intros)
+
+(*The set of all reachable states is an invariant...*)
+lemma invariant_reachable: "F : invariant (reachable F)"
+apply (simp add: invariant_def)
+apply (blast intro: reachable.intros)
+done
+
+(*...in fact the strongest invariant!*)
+lemma invariant_includes_reachable: "F : invariant A ==> reachable F <= A"
+apply (simp add: stable_def constrains_def invariant_def)
+apply (rule subsetI)
+apply (erule reachable.induct)
+apply (blast intro: reachable.intros)+
+done
+
+
+(*** Co ***)
+
+(*F : B co B' ==> F : (reachable F Int B) co (reachable F Int B')*)
+lemmas constrains_reachable_Int =  
+    subset_refl [THEN stable_reachable [unfolded stable_def], 
+                 THEN constrains_Int, standard]
+
+(*Resembles the previous definition of Constrains*)
+lemma Constrains_eq_constrains: 
+     "A Co B = {F. F : (reachable F  Int  A) co (reachable F  Int  B)}"
+apply (unfold Constrains_def)
+apply (blast dest: constrains_reachable_Int intro: constrains_weaken)
+done
+
+lemma constrains_imp_Constrains: "F : A co A' ==> F : A Co A'"
+apply (unfold Constrains_def)
+apply (blast intro: constrains_weaken_L)
+done
+
+lemma stable_imp_Stable: "F : stable A ==> F : Stable A"
+apply (unfold stable_def Stable_def)
+apply (erule constrains_imp_Constrains)
+done
+
+lemma ConstrainsI: 
+    "(!!act s s'. [| act: Acts F;  (s,s') : act;  s: A |] ==> s': A')  
+     ==> F : A Co A'"
+apply (rule constrains_imp_Constrains)
+apply (blast intro: constrainsI)
+done
+
+lemma Constrains_empty [iff]: "F : {} Co B"
+by (unfold Constrains_def constrains_def, blast)
+
+lemma Constrains_UNIV [iff]: "F : A Co UNIV"
+by (blast intro: ConstrainsI)
+
+lemma Constrains_weaken_R: 
+    "[| F : A Co A'; A'<=B' |] ==> F : A Co B'"
+apply (unfold Constrains_def)
+apply (blast intro: constrains_weaken_R)
+done
+
+lemma Constrains_weaken_L: 
+    "[| F : A Co A'; B<=A |] ==> F : B Co A'"
+apply (unfold Constrains_def)
+apply (blast intro: constrains_weaken_L)
+done
+
+lemma Constrains_weaken: 
+   "[| F : A Co A'; B<=A; A'<=B' |] ==> F : B Co B'"
+apply (unfold Constrains_def)
+apply (blast intro: constrains_weaken)
+done
+
+(** Union **)
+
+lemma Constrains_Un: 
+    "[| F : A Co A'; F : B Co B' |] ==> F : (A Un B) Co (A' Un B')"
+apply (unfold Constrains_def)
+apply (blast intro: constrains_Un [THEN constrains_weaken])
+done
+
+lemma Constrains_UN: 
+  assumes Co: "!!i. i:I ==> F : (A i) Co (A' i)"
+  shows "F : (UN i:I. A i) Co (UN i:I. A' i)"
+apply (unfold Constrains_def)
+apply (rule CollectI)
+apply (rule Co [unfolded Constrains_def, THEN CollectD, THEN constrains_UN, 
+                THEN constrains_weaken],   auto)
+done
+
+(** Intersection **)
+
+lemma Constrains_Int: 
+    "[| F : A Co A'; F : B Co B' |] ==> F : (A Int B) Co (A' Int B')"
+apply (unfold Constrains_def)
+apply (blast intro: constrains_Int [THEN constrains_weaken])
+done
+
+lemma Constrains_INT: 
+  assumes Co: "!!i. i:I ==> F : (A i) Co (A' i)"
+  shows "F : (INT i:I. A i) Co (INT i:I. A' i)"
+apply (unfold Constrains_def)
+apply (rule CollectI)
+apply (rule Co [unfolded Constrains_def, THEN CollectD, THEN constrains_INT, 
+                THEN constrains_weaken],   auto)
+done
+
+lemma Constrains_imp_subset: "F : A Co A' ==> reachable F Int A <= A'"
+by (simp add: constrains_imp_subset Constrains_def)
+
+lemma Constrains_trans: "[| F : A Co B; F : B Co C |] ==> F : A Co C"
+apply (simp add: Constrains_eq_constrains)
+apply (blast intro: constrains_trans constrains_weaken)
+done
+
+lemma Constrains_cancel:
+     "[| F : A Co (A' Un B); F : B Co B' |] ==> F : A Co (A' Un B')"
+by (simp add: Constrains_eq_constrains constrains_def, blast)
+
+
+(*** Stable ***)
+
+(*Useful because there's no Stable_weaken.  [Tanja Vos]*)
+lemma Stable_eq: "[| F: Stable A; A = B |] ==> F : Stable B"
+by blast
+
+lemma Stable_eq_stable: "(F : Stable A) = (F : stable (reachable F Int A))"
+by (simp add: Stable_def Constrains_eq_constrains stable_def)
+
+lemma StableI: "F : A Co A ==> F : Stable A"
+by (unfold Stable_def, assumption)
+
+lemma StableD: "F : Stable A ==> F : A Co A"
+by (unfold Stable_def, assumption)
+
+lemma Stable_Un: 
+    "[| F : Stable A; F : Stable A' |] ==> F : Stable (A Un A')"
+apply (unfold Stable_def)
+apply (blast intro: Constrains_Un)
+done
+
+lemma Stable_Int: 
+    "[| F : Stable A; F : Stable A' |] ==> F : Stable (A Int A')"
+apply (unfold Stable_def)
+apply (blast intro: Constrains_Int)
+done
+
+lemma Stable_Constrains_Un: 
+    "[| F : Stable C; F : A Co (C Un A') |]    
+     ==> F : (C Un A) Co (C Un A')"
+apply (unfold Stable_def)
+apply (blast intro: Constrains_Un [THEN Constrains_weaken])
+done
+
+lemma Stable_Constrains_Int: 
+    "[| F : Stable C; F : (C Int A) Co A' |]    
+     ==> F : (C Int A) Co (C Int A')"
+apply (unfold Stable_def)
+apply (blast intro: Constrains_Int [THEN Constrains_weaken])
+done
+
+lemma Stable_UN: 
+    "(!!i. i:I ==> F : Stable (A i)) ==> F : Stable (UN i:I. A i)"
+by (simp add: Stable_def Constrains_UN) 
+
+lemma Stable_INT: 
+    "(!!i. i:I ==> F : Stable (A i)) ==> F : Stable (INT i:I. A i)"
+by (simp add: Stable_def Constrains_INT) 
+
+lemma Stable_reachable: "F : Stable (reachable F)"
+by (simp add: Stable_eq_stable)
+
+
+
+(*** Increasing ***)
+
+lemma IncreasingD: 
+     "F : Increasing f ==> F : Stable {s. x <= f s}"
+by (unfold Increasing_def, blast)
+
+lemma mono_Increasing_o: 
+     "mono g ==> Increasing f <= Increasing (g o f)"
+apply (simp add: Increasing_def Stable_def Constrains_def stable_def 
+                 constrains_def)
+apply (blast intro: monoD order_trans)
+done
+
+lemma strict_IncreasingD: 
+     "!!z::nat. F : Increasing f ==> F: Stable {s. z < f s}"
+by (simp add: Increasing_def Suc_le_eq [symmetric])
+
+lemma increasing_imp_Increasing: 
+     "F : increasing f ==> F : Increasing f"
+apply (unfold increasing_def Increasing_def)
+apply (blast intro: stable_imp_Stable)
+done
+
+lemmas Increasing_constant =  
+    increasing_constant [THEN increasing_imp_Increasing, standard, iff]
+
+
+(*** The Elimination Theorem.  The "free" m has become universally quantified!
+     Should the premise be !!m instead of ALL m ?  Would make it harder to use
+     in forward proof. ***)
+
+lemma Elimination: 
+    "[| ALL m. F : {s. s x = m} Co (B m) |]  
+     ==> F : {s. s x : M} Co (UN m:M. B m)"
+
+by (unfold Constrains_def constrains_def, blast)
+
+(*As above, but for the trivial case of a one-variable state, in which the
+  state is identified with its one variable.*)
+lemma Elimination_sing: 
+    "(ALL m. F : {m} Co (B m)) ==> F : M Co (UN m:M. B m)"
+by (unfold Constrains_def constrains_def, blast)
+
+
+(*** Specialized laws for handling Always ***)
+
+(** Natural deduction rules for "Always A" **)
+
+lemma AlwaysI: "[| Init F<=A;  F : Stable A |] ==> F : Always A"
+by (simp add: Always_def)
+
+lemma AlwaysD: "F : Always A ==> Init F<=A & F : Stable A"
+by (simp add: Always_def)
+
+lemmas AlwaysE = AlwaysD [THEN conjE, standard]
+lemmas Always_imp_Stable = AlwaysD [THEN conjunct2, standard]
+
+
+(*The set of all reachable states is Always*)
+lemma Always_includes_reachable: "F : Always A ==> reachable F <= A"
+apply (simp add: Stable_def Constrains_def constrains_def Always_def)
+apply (rule subsetI)
+apply (erule reachable.induct)
+apply (blast intro: reachable.intros)+
+done
+
+lemma invariant_imp_Always: 
+     "F : invariant A ==> F : Always A"
+apply (unfold Always_def invariant_def Stable_def stable_def)
+apply (blast intro: constrains_imp_Constrains)
+done
+
+lemmas Always_reachable =
+    invariant_reachable [THEN invariant_imp_Always, standard]
+
+lemma Always_eq_invariant_reachable:
+     "Always A = {F. F : invariant (reachable F Int A)}"
+apply (simp add: Always_def invariant_def Stable_def Constrains_eq_constrains
+                 stable_def)
+apply (blast intro: reachable.intros)
+done
+
+(*the RHS is the traditional definition of the "always" operator*)
+lemma Always_eq_includes_reachable: "Always A = {F. reachable F <= A}"
+by (auto dest: invariant_includes_reachable simp add: Int_absorb2 invariant_reachable Always_eq_invariant_reachable)
+
+lemma Always_UNIV_eq [simp]: "Always UNIV = UNIV"
+by (auto simp add: Always_eq_includes_reachable)
+
+lemma UNIV_AlwaysI: "UNIV <= A ==> F : Always A"
+by (auto simp add: Always_eq_includes_reachable)
+
+lemma Always_eq_UN_invariant: "Always A = (UN I: Pow A. invariant I)"
+apply (simp add: Always_eq_includes_reachable)
+apply (blast intro: invariantI Init_subset_reachable [THEN subsetD] 
+                    invariant_includes_reachable [THEN subsetD])
+done
+
+lemma Always_weaken: "[| F : Always A; A <= B |] ==> F : Always B"
+by (auto simp add: Always_eq_includes_reachable)
+
+
+(*** "Co" rules involving Always ***)
+
+lemma Always_Constrains_pre:
+     "F : Always INV ==> (F : (INV Int A) Co A') = (F : A Co A')"
+by (simp add: Always_includes_reachable [THEN Int_absorb2] Constrains_def 
+              Int_assoc [symmetric])
+
+lemma Always_Constrains_post:
+     "F : Always INV ==> (F : A Co (INV Int A')) = (F : A Co A')"
+by (simp add: Always_includes_reachable [THEN Int_absorb2] 
+              Constrains_eq_constrains Int_assoc [symmetric])
+
+(* [| F : Always INV;  F : (INV Int A) Co A' |] ==> F : A Co A' *)
+lemmas Always_ConstrainsI = Always_Constrains_pre [THEN iffD1, standard]
+
+(* [| F : Always INV;  F : A Co A' |] ==> F : A Co (INV Int A') *)
+lemmas Always_ConstrainsD = Always_Constrains_post [THEN iffD2, standard]
+
+(*The analogous proof of Always_LeadsTo_weaken doesn't terminate*)
+lemma Always_Constrains_weaken:
+     "[| F : Always C;  F : A Co A';    
+         C Int B <= A;   C Int A' <= B' |]  
+      ==> F : B Co B'"
+apply (rule Always_ConstrainsI, assumption)
+apply (drule Always_ConstrainsD, assumption)
+apply (blast intro: Constrains_weaken)
+done
+
+
+(** Conjoining Always properties **)
+
+lemma Always_Int_distrib: "Always (A Int B) = Always A Int Always B"
+by (auto simp add: Always_eq_includes_reachable)
+
+lemma Always_INT_distrib: "Always (INTER I A) = (INT i:I. Always (A i))"
+by (auto simp add: Always_eq_includes_reachable)
+
+lemma Always_Int_I:
+     "[| F : Always A;  F : Always B |] ==> F : Always (A Int B)"
+by (simp add: Always_Int_distrib)
+
+(*Allows a kind of "implication introduction"*)
+lemma Always_Compl_Un_eq:
+     "F : Always A ==> (F : Always (-A Un B)) = (F : Always B)"
+by (auto simp add: Always_eq_includes_reachable)
+
+(*Delete the nearest invariance assumption (which will be the second one
+  used by Always_Int_I) *)
+lemmas Always_thin = thin_rl [of "F : Always A", standard]
 
 end
