src/HOL/UNITY/WFair.thy
@@ -8,7 +8,7 @@ Weak Fairness versions of transient, ensures, leadsTo.
 From Misra, "A Logic for Concurrent Programming", 1994
 *)
 
-WFair = UNITY +
+theory WFair = UNITY:
 
 constdefs
 
@@ -17,7 +17,7 @@ constdefs
   transient :: "'a set => 'a program set"
     "transient A == {F. EX act: Acts F. A <= Domain act & act``A <= -A}"
 
-  ensures :: "['a set, 'a set] => 'a program set"       (infixl 60)
+  ensures :: "['a set, 'a set] => 'a program set"       (infixl "ensures" 60)
     "A ensures B == (A-B co A Un B) Int transient (A-B)"
 
 
@@ -28,19 +28,19 @@ consts
 
 
 inductive "leads F"
-  intrs 
+  intros 
 
-    Basis  "F : A ensures B ==> (A,B) : leads F"
+    Basis:  "F : A ensures B ==> (A,B) : leads F"
 
-    Trans  "[| (A,B) : leads F;  (B,C) : leads F |] ==> (A,C) : leads F"
+    Trans:  "[| (A,B) : leads F;  (B,C) : leads F |] ==> (A,C) : leads F"
 
-    Union  "ALL A: S. (A,B) : leads F ==> (Union S, B) : leads F"
+    Union:  "ALL A: S. (A,B) : leads F ==> (Union S, B) : leads F"
 
 
 constdefs
 
   (*visible version of the LEADS-TO relation*)
-  leadsTo :: "['a set, 'a set] => 'a program set"       (infixl 60)
+  leadsTo :: "['a set, 'a set] => 'a program set"    (infixl "leadsTo" 60)
     "A leadsTo B == {F. (A,B) : leads F}"
   
   (*wlt F B is the largest set that leads to B*)
@@ -48,6 +48,537 @@ constdefs
     "wlt F B == Union {A. F: A leadsTo B}"
 
 syntax (xsymbols)
-  "op leadsTo" :: "['a set, 'a set] => 'a program set" (infixl "\\<longmapsto>" 60)
+  "op leadsTo" :: "['a set, 'a set] => 'a program set" (infixl "\<longmapsto>" 60)
+
+
+(*** transient ***)
+
+lemma stable_transient_empty: 
+    "[| F : stable A; F : transient A |] ==> A = {}"
+
+by (unfold stable_def constrains_def transient_def, blast)
+
+lemma transient_strengthen: 
+    "[| F : transient A; B<=A |] ==> F : transient B"
+apply (unfold transient_def, clarify)
+apply (blast intro!: rev_bexI)
+done
+
+lemma transientI: 
+    "[| act: Acts F;  A <= Domain act;  act``A <= -A |] ==> F : transient A"
+by (unfold transient_def, blast)
+
+lemma transientE: 
+    "[| F : transient A;   
+        !!act. [| act: Acts F;  A <= Domain act;  act``A <= -A |] ==> P |]  
+     ==> P"
+by (unfold transient_def, blast)
+
+lemma transient_UNIV [simp]: "transient UNIV = {}"
+by (unfold transient_def, blast)
+
+lemma transient_empty [simp]: "transient {} = UNIV"
+by (unfold transient_def, auto)
+
+
+(*** ensures ***)
+
+lemma ensuresI: 
+    "[| F : (A-B) co (A Un B); F : transient (A-B) |] ==> F : A ensures B"
+by (unfold ensures_def, blast)
+
+lemma ensuresD: 
+    "F : A ensures B ==> F : (A-B) co (A Un B) & F : transient (A-B)"
+by (unfold ensures_def, blast)
+
+lemma ensures_weaken_R: 
+    "[| F : A ensures A'; A'<=B' |] ==> F : A ensures B'"
+apply (unfold ensures_def)
+apply (blast intro: constrains_weaken transient_strengthen)
+done
+
+(*The L-version (precondition strengthening) fails, but we have this*)
+lemma stable_ensures_Int: 
+    "[| F : stable C;  F : A ensures B |]    
+    ==> F : (C Int A) ensures (C Int B)"
+apply (unfold ensures_def)
+apply (auto simp add: ensures_def Int_Un_distrib [symmetric] Diff_Int_distrib [symmetric])
+prefer 2 apply (blast intro: transient_strengthen)
+apply (blast intro: stable_constrains_Int constrains_weaken)
+done
+
+lemma stable_transient_ensures:
+     "[| F : stable A;  F : transient C;  A <= B Un C |] ==> F : A ensures B"
+apply (simp add: ensures_def stable_def)
+apply (blast intro: constrains_weaken transient_strengthen)
+done
+
+lemma ensures_eq: "(A ensures B) = (A unless B) Int transient (A-B)"
+by (simp (no_asm) add: ensures_def unless_def)
+
+
+(*** leadsTo ***)
+
+lemma leadsTo_Basis [intro]: "F : A ensures B ==> F : A leadsTo B"
+apply (unfold leadsTo_def)
+apply (blast intro: leads.Basis)
+done
+
+lemma leadsTo_Trans: 
+     "[| F : A leadsTo B;  F : B leadsTo C |] ==> F : A leadsTo C"
+apply (unfold leadsTo_def)
+apply (blast intro: leads.Trans)
+done
+
+lemma transient_imp_leadsTo: "F : transient A ==> F : A leadsTo (-A)"
+by (simp (no_asm_simp) add: leadsTo_Basis ensuresI Compl_partition)
+
+(*Useful with cancellation, disjunction*)
+lemma leadsTo_Un_duplicate: "F : A leadsTo (A' Un A') ==> F : A leadsTo A'"
+by (simp add: Un_ac)
+
+lemma leadsTo_Un_duplicate2:
+     "F : A leadsTo (A' Un C Un C) ==> F : A leadsTo (A' Un C)"
+by (simp add: Un_ac)
+
+(*The Union introduction rule as we should have liked to state it*)
+lemma leadsTo_Union: 
+    "(!!A. A : S ==> F : A leadsTo B) ==> F : (Union S) leadsTo B"
+apply (unfold leadsTo_def)
+apply (blast intro: leads.Union)
+done
+
+lemma leadsTo_Union_Int: 
+ "(!!A. A : S ==> F : (A Int C) leadsTo B) ==> F : (Union S Int C) leadsTo B"
+apply (unfold leadsTo_def)
+apply (simp only: Int_Union_Union)
+apply (blast intro: leads.Union)
+done
+
+lemma leadsTo_UN: 
+    "(!!i. i : I ==> F : (A i) leadsTo B) ==> F : (UN i:I. A i) leadsTo B"
+apply (subst Union_image_eq [symmetric])
+apply (blast intro: leadsTo_Union)
+done
+
+(*Binary union introduction rule*)
+lemma leadsTo_Un:
+     "[| F : A leadsTo C; F : B leadsTo C |] ==> F : (A Un B) leadsTo C"
+apply (subst Un_eq_Union)
+apply (blast intro: leadsTo_Union)
+done
+
+lemma single_leadsTo_I: 
+     "(!!x. x : A ==> F : {x} leadsTo B) ==> F : A leadsTo B"
+by (subst UN_singleton [symmetric], rule leadsTo_UN, blast)
+
+
+(*The INDUCTION rule as we should have liked to state it*)
+lemma leadsTo_induct: 
+  "[| F : za leadsTo zb;   
+      !!A B. F : A ensures B ==> P A B;  
+      !!A B C. [| F : A leadsTo B; P A B; F : B leadsTo C; P B C |]  
+               ==> P A C;  
+      !!B S. ALL A:S. F : A leadsTo B & P A B ==> P (Union S) B  
+   |] ==> P za zb"
+apply (unfold leadsTo_def)
+apply (drule CollectD, erule leads.induct)
+apply (blast+)
+done
+
+
+lemma subset_imp_ensures: "A<=B ==> F : A ensures B"
+by (unfold ensures_def constrains_def transient_def, blast)
+
+lemmas subset_imp_leadsTo = subset_imp_ensures [THEN leadsTo_Basis, standard]
+
+lemmas leadsTo_refl = subset_refl [THEN subset_imp_leadsTo, standard]
+
+lemmas empty_leadsTo = empty_subsetI [THEN subset_imp_leadsTo, standard, simp]
+
+lemmas leadsTo_UNIV = subset_UNIV [THEN subset_imp_leadsTo, standard, simp]
+
+
+
+(** Variant induction rule: on the preconditions for B **)
+
+(*Lemma is the weak version: can't see how to do it in one step*)
+lemma leadsTo_induct_pre_lemma: 
+  "[| F : za leadsTo zb;   
+      P zb;  
+      !!A B. [| F : A ensures B;  P B |] ==> P A;  
+      !!S. ALL A:S. P A ==> P (Union S)  
+   |] ==> P za"
+(*by induction on this formula*)
+apply (subgoal_tac "P zb --> P za")
+(*now solve first subgoal: this formula is sufficient*)
+apply (blast intro: leadsTo_refl)
+apply (erule leadsTo_induct)
+apply (blast+)
+done
+
+lemma leadsTo_induct_pre: 
+  "[| F : za leadsTo zb;   
+      P zb;  
+      !!A B. [| F : A ensures B;  F : B leadsTo zb;  P B |] ==> P A;  
+      !!S. ALL A:S. F : A leadsTo zb & P A ==> P (Union S)  
+   |] ==> P za"
+apply (subgoal_tac "F : za leadsTo zb & P za")
+apply (erule conjunct2)
+apply (erule leadsTo_induct_pre_lemma)
+prefer 3 apply (blast intro: leadsTo_Union)
+prefer 2 apply (blast intro: leadsTo_Trans)
+apply (blast intro: leadsTo_refl)
+done
+
+
+lemma leadsTo_weaken_R: "[| F : A leadsTo A'; A'<=B' |] ==> F : A leadsTo B'"
+by (blast intro: subset_imp_leadsTo leadsTo_Trans)
+
+lemma leadsTo_weaken_L [rule_format (no_asm)]:
+     "[| F : A leadsTo A'; B<=A |] ==> F : B leadsTo A'"
+by (blast intro: leadsTo_Trans subset_imp_leadsTo)
+
+(*Distributes over binary unions*)
+lemma leadsTo_Un_distrib:
+     "F : (A Un B) leadsTo C  =  (F : A leadsTo C & F : B leadsTo C)"
+by (blast intro: leadsTo_Un leadsTo_weaken_L)
+
+lemma leadsTo_UN_distrib:
+     "F : (UN i:I. A i) leadsTo B  =  (ALL i : I. F : (A i) leadsTo B)"
+by (blast intro: leadsTo_UN leadsTo_weaken_L)
+
+lemma leadsTo_Union_distrib:
+     "F : (Union S) leadsTo B  =  (ALL A : S. F : A leadsTo B)"
+by (blast intro: leadsTo_Union leadsTo_weaken_L)
+
+
+lemma leadsTo_weaken:
+     "[| F : A leadsTo A'; B<=A; A'<=B' |] ==> F : B leadsTo B'"
+by (blast intro: leadsTo_weaken_R leadsTo_weaken_L leadsTo_Trans)
+
+
+(*Set difference: maybe combine with leadsTo_weaken_L?*)
+lemma leadsTo_Diff:
+     "[| F : (A-B) leadsTo C; F : B leadsTo C |]   ==> F : A leadsTo C"
+by (blast intro: leadsTo_Un leadsTo_weaken)
+
+lemma leadsTo_UN_UN:
+   "(!! i. i:I ==> F : (A i) leadsTo (A' i))  
+    ==> F : (UN i:I. A i) leadsTo (UN i:I. A' i)"
+apply (simp only: Union_image_eq [symmetric])
+apply (blast intro: leadsTo_Union leadsTo_weaken_R)
+done
+
+(*Binary union version*)
+lemma leadsTo_Un_Un:
+     "[| F : A leadsTo A'; F : B leadsTo B' |]  
+      ==> F : (A Un B) leadsTo (A' Un B')"
+by (blast intro: leadsTo_Un leadsTo_weaken_R)
+
+
+(** The cancellation law **)
+
+lemma leadsTo_cancel2:
+     "[| F : A leadsTo (A' Un B); F : B leadsTo B' |]  
+      ==> F : A leadsTo (A' Un B')"
+by (blast intro: leadsTo_Un_Un subset_imp_leadsTo leadsTo_Trans)
+
+lemma leadsTo_cancel_Diff2:
+     "[| F : A leadsTo (A' Un B); F : (B-A') leadsTo B' |]  
+      ==> F : A leadsTo (A' Un B')"
+apply (rule leadsTo_cancel2)
+prefer 2 apply assumption
+apply (simp_all (no_asm_simp))
+done
+
+lemma leadsTo_cancel1:
+     "[| F : A leadsTo (B Un A'); F : B leadsTo B' |]  
+    ==> F : A leadsTo (B' Un A')"
+apply (simp add: Un_commute)
+apply (blast intro!: leadsTo_cancel2)
+done
+
+lemma leadsTo_cancel_Diff1:
+     "[| F : A leadsTo (B Un A'); F : (B-A') leadsTo B' |]  
+    ==> F : A leadsTo (B' Un A')"
+apply (rule leadsTo_cancel1)
+prefer 2 apply assumption
+apply (simp_all (no_asm_simp))
+done
+
+
+
+(** The impossibility law **)
+
+lemma leadsTo_empty: "F : A leadsTo {} ==> A={}"
+apply (erule leadsTo_induct_pre)
+apply (simp_all add: ensures_def constrains_def transient_def, blast)
+done
+
+
+(** PSP: Progress-Safety-Progress **)
+
+(*Special case of PSP: Misra's "stable conjunction"*)
+lemma psp_stable: 
+   "[| F : A leadsTo A'; F : stable B |]  
+    ==> F : (A Int B) leadsTo (A' Int B)"
+apply (unfold stable_def)
+apply (erule leadsTo_induct)
+prefer 3 apply (blast intro: leadsTo_Union_Int)
+prefer 2 apply (blast intro: leadsTo_Trans)
+apply (rule leadsTo_Basis)
+apply (simp add: ensures_def Diff_Int_distrib2 [symmetric] Int_Un_distrib2 [symmetric])
+apply (blast intro: transient_strengthen constrains_Int)
+done
+
+lemma psp_stable2: 
+   "[| F : A leadsTo A'; F : stable B |] ==> F : (B Int A) leadsTo (B Int A')"
+by (simp add: psp_stable Int_ac)
+
+lemma psp_ensures: 
+   "[| F : A ensures A'; F : B co B' |]  
+    ==> F : (A Int B') ensures ((A' Int B) Un (B' - B))"
+apply (unfold ensures_def constrains_def, clarify) (*speeds up the proof*)
+apply (blast intro: transient_strengthen)
+done
+
+lemma psp:
+     "[| F : A leadsTo A'; F : B co B' |]  
+      ==> F : (A Int B') leadsTo ((A' Int B) Un (B' - B))"
+apply (erule leadsTo_induct)
+  prefer 3 apply (blast intro: leadsTo_Union_Int)
+ txt{*Basis case*}
+ apply (blast intro: psp_ensures)
+txt{*Transitivity case has a delicate argument involving "cancellation"*}
+apply (rule leadsTo_Un_duplicate2)
+apply (erule leadsTo_cancel_Diff1)
+apply (simp add: Int_Diff Diff_triv)
+apply (blast intro: leadsTo_weaken_L dest: constrains_imp_subset)
+done
+
+lemma psp2:
+     "[| F : A leadsTo A'; F : B co B' |]  
+    ==> F : (B' Int A) leadsTo ((B Int A') Un (B' - B))"
+by (simp (no_asm_simp) add: psp Int_ac)
+
+lemma psp_unless: 
+   "[| F : A leadsTo A';  F : B unless B' |]  
+    ==> F : (A Int B) leadsTo ((A' Int B) Un B')"
+
+apply (unfold unless_def)
+apply (drule psp, assumption)
+apply (blast intro: leadsTo_weaken)
+done
+
+
+(*** Proving the induction rules ***)
+
+(** The most general rule: r is any wf relation; f is any variant function **)
+
+lemma leadsTo_wf_induct_lemma:
+     "[| wf r;      
+         ALL m. F : (A Int f-`{m}) leadsTo                      
+                    ((A Int f-`(r^-1 `` {m})) Un B) |]  
+      ==> F : (A Int f-`{m}) leadsTo B"
+apply (erule_tac a = m in wf_induct)
+apply (subgoal_tac "F : (A Int (f -` (r^-1 `` {x}))) leadsTo B")
+ apply (blast intro: leadsTo_cancel1 leadsTo_Un_duplicate)
+apply (subst vimage_eq_UN)
+apply (simp only: UN_simps [symmetric])
+apply (blast intro: leadsTo_UN)
+done
+
+
+(** Meta or object quantifier ? **)
+lemma leadsTo_wf_induct:
+     "[| wf r;      
+         ALL m. F : (A Int f-`{m}) leadsTo                      
+                    ((A Int f-`(r^-1 `` {m})) Un B) |]  
+      ==> F : A leadsTo B"
+apply (rule_tac t = A in subst)
+ defer 1
+ apply (rule leadsTo_UN)
+ apply (erule leadsTo_wf_induct_lemma)
+ apply assumption
+apply fast (*Blast_tac: Function unknown's argument not a parameter*)
+done
+
+
+lemma bounded_induct:
+     "[| wf r;      
+         ALL m:I. F : (A Int f-`{m}) leadsTo                    
+                      ((A Int f-`(r^-1 `` {m})) Un B) |]  
+      ==> F : A leadsTo ((A - (f-`I)) Un B)"
+apply (erule leadsTo_wf_induct, safe)
+apply (case_tac "m:I")
+apply (blast intro: leadsTo_weaken)
+apply (blast intro: subset_imp_leadsTo)
+done
+
+
+(*Alternative proof is via the lemma F : (A Int f-`(lessThan m)) leadsTo B*)
+lemma lessThan_induct: 
+     "[| !!m::nat. F : (A Int f-`{m}) leadsTo ((A Int f-`{..m(}) Un B) |]  
+      ==> F : A leadsTo B"
+apply (rule wf_less_than [THEN leadsTo_wf_induct])
+apply (simp (no_asm_simp))
+apply blast
+done
+
+lemma lessThan_bounded_induct:
+     "!!l::nat. [| ALL m:(greaterThan l).     
+            F : (A Int f-`{m}) leadsTo ((A Int f-`(lessThan m)) Un B) |]  
+      ==> F : A leadsTo ((A Int (f-`(atMost l))) Un B)"
+apply (simp only: Diff_eq [symmetric] vimage_Compl Compl_greaterThan [symmetric])
+apply (rule wf_less_than [THEN bounded_induct])
+apply (simp (no_asm_simp))
+done
+
+lemma greaterThan_bounded_induct:
+     "!!l::nat. [| ALL m:(lessThan l).     
+            F : (A Int f-`{m}) leadsTo ((A Int f-`(greaterThan m)) Un B) |]  
+      ==> F : A leadsTo ((A Int (f-`(atLeast l))) Un B)"
+apply (rule_tac f = f and f1 = "%k. l - k" 
+       in wf_less_than [THEN wf_inv_image, THEN leadsTo_wf_induct])
+apply (simp (no_asm) add: inv_image_def Image_singleton)
+apply clarify
+apply (case_tac "m<l")
+prefer 2 apply (blast intro: not_leE subset_imp_leadsTo)
+apply (blast intro: leadsTo_weaken_R diff_less_mono2)
+done
+
+
+(*** wlt ****)
+
+(*Misra's property W3*)
+lemma wlt_leadsTo: "F : (wlt F B) leadsTo B"
+apply (unfold wlt_def)
+apply (blast intro!: leadsTo_Union)
+done
+
+lemma leadsTo_subset: "F : A leadsTo B ==> A <= wlt F B"
+apply (unfold wlt_def)
+apply (blast intro!: leadsTo_Union)
+done
+
+(*Misra's property W2*)
+lemma leadsTo_eq_subset_wlt: "F : A leadsTo B = (A <= wlt F B)"
+by (blast intro!: leadsTo_subset wlt_leadsTo [THEN leadsTo_weaken_L])
+
+(*Misra's property W4*)
+lemma wlt_increasing: "B <= wlt F B"
+apply (simp (no_asm_simp) add: leadsTo_eq_subset_wlt [symmetric] subset_imp_leadsTo)
+done
+
+
+(*Used in the Trans case below*)
+lemma lemma1: 
+   "[| B <= A2;   
+       F : (A1 - B) co (A1 Un B);  
+       F : (A2 - C) co (A2 Un C) |]  
+    ==> F : (A1 Un A2 - C) co (A1 Un A2 Un C)"
+by (unfold constrains_def, clarify,  blast)
+
+(*Lemma (1,2,3) of Misra's draft book, Chapter 4, "Progress"*)
+lemma leadsTo_123:
+     "F : A leadsTo A'  
+      ==> EX B. A<=B & F : B leadsTo A' & F : (B-A') co (B Un A')"
+apply (erule leadsTo_induct)
+(*Basis*)
+apply (blast dest: ensuresD)
+(*Trans*)
+apply clarify
+apply (rule_tac x = "Ba Un Bb" in exI)
+apply (blast intro: lemma1 leadsTo_Un_Un leadsTo_cancel1 leadsTo_Un_duplicate)
+(*Union*)
+apply (clarify dest!: ball_conj_distrib [THEN iffD1] bchoice)
+apply (rule_tac x = "UN A:S. f A" in exI)
+apply (auto intro: leadsTo_UN)
+(*Blast_tac says PROOF FAILED*)
+apply (rule_tac I1=S and A1="%i. f i - B" and A'1="%i. f i Un B" 
+       in constrains_UN [THEN constrains_weaken])
+apply (auto ); 
+done
+
+
+(*Misra's property W5*)
+lemma wlt_constrains_wlt: "F : (wlt F B - B) co (wlt F B)"
+apply (cut_tac F = F in wlt_leadsTo [THEN leadsTo_123], clarify)
+apply (subgoal_tac "Ba = wlt F B")
+prefer 2 apply (blast dest: leadsTo_eq_subset_wlt [THEN iffD1], clarify)
+apply (simp add: wlt_increasing Un_absorb2)
+done
+
+
+(*** Completion: Binary and General Finite versions ***)
+
+lemma completion_lemma :
+     "[| W = wlt F (B' Un C);      
+       F : A leadsTo (A' Un C);  F : A' co (A' Un C);    
+       F : B leadsTo (B' Un C);  F : B' co (B' Un C) |]  
+    ==> F : (A Int B) leadsTo ((A' Int B') Un C)"
+apply (subgoal_tac "F : (W-C) co (W Un B' Un C) ")
+ prefer 2
+ apply (blast intro: wlt_constrains_wlt [THEN [2] constrains_Un, 
+                                         THEN constrains_weaken])
+apply (subgoal_tac "F : (W-C) co W")
+ prefer 2
+ apply (simp add: wlt_increasing Un_assoc Un_absorb2)
+apply (subgoal_tac "F : (A Int W - C) leadsTo (A' Int W Un C) ")
+ prefer 2 apply (blast intro: wlt_leadsTo psp [THEN leadsTo_weaken])
+(** LEVEL 6 **)
+apply (subgoal_tac "F : (A' Int W Un C) leadsTo (A' Int B' Un C) ")
+ prefer 2
+ apply (rule leadsTo_Un_duplicate2)
+ apply (blast intro: leadsTo_Un_Un wlt_leadsTo
+                         [THEN psp2, THEN leadsTo_weaken] leadsTo_refl)
+apply (drule leadsTo_Diff)
+apply (blast intro: subset_imp_leadsTo)
+apply (subgoal_tac "A Int B <= A Int W")
+ prefer 2
+ apply (blast dest!: leadsTo_subset intro!: subset_refl [THEN Int_mono])
+apply (blast intro: leadsTo_Trans subset_imp_leadsTo)
+done
+
+lemmas completion = completion_lemma [OF refl]
+
+lemma finite_completion_lemma:
+     "finite I ==> (ALL i:I. F : (A i) leadsTo (A' i Un C)) -->   
+                   (ALL i:I. F : (A' i) co (A' i Un C)) -->  
+                   F : (INT i:I. A i) leadsTo ((INT i:I. A' i) Un C)"
+apply (erule finite_induct, auto)
+apply (rule completion)
+   prefer 4
+   apply (simp only: INT_simps [symmetric])
+   apply (rule constrains_INT, auto)
+done
+
+lemma finite_completion: 
+     "[| finite I;   
+         !!i. i:I ==> F : (A i) leadsTo (A' i Un C);  
+         !!i. i:I ==> F : (A' i) co (A' i Un C) |]    
+      ==> F : (INT i:I. A i) leadsTo ((INT i:I. A' i) Un C)"
+by (blast intro: finite_completion_lemma [THEN mp, THEN mp])
+
+lemma stable_completion: 
+     "[| F : A leadsTo A';  F : stable A';    
+         F : B leadsTo B';  F : stable B' |]  
+    ==> F : (A Int B) leadsTo (A' Int B')"
+apply (unfold stable_def)
+apply (rule_tac C1 = "{}" in completion [THEN leadsTo_weaken_R])
+apply (force+)
+done
+
+lemma finite_stable_completion: 
+     "[| finite I;   
+         !!i. i:I ==> F : (A i) leadsTo (A' i);  
+         !!i. i:I ==> F : stable (A' i) |]    
+      ==> F : (INT i:I. A i) leadsTo (INT i:I. A' i)"
+apply (unfold stable_def)
+apply (rule_tac C1 = "{}" in finite_completion [THEN leadsTo_weaken_R])
+apply (simp_all (no_asm_simp))
+apply blast+
+done
 
 end
