src/HOL/UNITY/UNITY.thy
@@ -8,18 +8,21 @@ The basic UNITY theory (revised version, based upon the "co" operator)
 From Misra, "A Logic for Concurrent Programming", 1994
 *)
 
-UNITY = Main + 
+theory UNITY = Main:
 
 typedef (Program)
   'a program = "{(init:: 'a set, acts :: ('a * 'a)set set,
-		  allowed :: ('a * 'a)set set). Id:acts & Id: allowed}"
-
-consts
-  constrains :: "['a set, 'a set] => 'a program set"  (infixl "co"     60)
-  op_unless  :: "['a set, 'a set] => 'a program set"  (infixl "unless" 60)
+		   allowed :: ('a * 'a)set set). Id:acts & Id: allowed}" 
+  by blast
 
 constdefs
-    mk_program :: "('a set * ('a * 'a)set set * ('a * 'a)set set)
+  constrains :: "['a set, 'a set] => 'a program set"  (infixl "co"     60)
+    "A co B == {F. ALL act: Acts F. act``A <= B}"
+
+  unless  :: "['a set, 'a set] => 'a program set"  (infixl "unless" 60)
+    "A unless B == (A-B) co (A Un B)"
+
+  mk_program :: "('a set * ('a * 'a)set set * ('a * 'a)set set)
 		   => 'a program"
     "mk_program == %(init, acts, allowed).
                       Abs_Program (init, insert Id acts, insert Id allowed)"
@@ -50,9 +53,325 @@ constdefs
     "increasing f == INT z. stable {s. z <= f s}"
 
 
-defs
-  constrains_def "A co B == {F. ALL act: Acts F. act``A <= B}"
+(*Perhaps equalities.ML shouldn't add this in the first place!*)
+declare image_Collect [simp del]
 
-  unless_def     "A unless B == (A-B) co (A Un B)"
+(*** The abstract type of programs ***)
+
+lemmas program_typedef =
+     Rep_Program Rep_Program_inverse Abs_Program_inverse 
+     Program_def Init_def Acts_def AllowedActs_def mk_program_def
+
+lemma Id_in_Acts [iff]: "Id : Acts F"
+apply (cut_tac x = F in Rep_Program)
+apply (auto simp add: program_typedef) 
+done
+
+lemma insert_Id_Acts [iff]: "insert Id (Acts F) = Acts F"
+by (simp add: insert_absorb Id_in_Acts)
+
+lemma Id_in_AllowedActs [iff]: "Id : AllowedActs F"
+apply (cut_tac x = F in Rep_Program)
+apply (auto simp add: program_typedef) 
+done
+
+lemma insert_Id_AllowedActs [iff]: "insert Id (AllowedActs F) = AllowedActs F"
+by (simp add: insert_absorb Id_in_AllowedActs)
+
+(** Inspectors for type "program" **)
+
+lemma Init_eq [simp]: "Init (mk_program (init,acts,allowed)) = init"
+by (auto simp add: program_typedef)
+
+lemma Acts_eq [simp]: "Acts (mk_program (init,acts,allowed)) = insert Id acts"
+by (auto simp add: program_typedef)
+
+lemma AllowedActs_eq [simp]:
+     "AllowedActs (mk_program (init,acts,allowed)) = insert Id allowed"
+by (auto simp add: program_typedef)
+
+(** Equality for UNITY programs **)
+
+lemma surjective_mk_program [simp]:
+     "mk_program (Init F, Acts F, AllowedActs F) = F"
+apply (cut_tac x = F in Rep_Program)
+apply (auto simp add: program_typedef)
+apply (drule_tac f = Abs_Program in arg_cong)+
+apply (simp add: program_typedef insert_absorb)
+done
+
+lemma program_equalityI:
+     "[| Init F = Init G; Acts F = Acts G; AllowedActs F = AllowedActs G |]  
+      ==> F = G"
+apply (rule_tac t = F in surjective_mk_program [THEN subst])
+apply (rule_tac t = G in surjective_mk_program [THEN subst], simp)
+done
+
+lemma program_equalityE:
+     "[| F = G;  
+         [| Init F = Init G; Acts F = Acts G; AllowedActs F = AllowedActs G |] 
+         ==> P |] ==> P"
+by simp 
+
+lemma program_equality_iff:
+     "(F=G) =   
+      (Init F = Init G & Acts F = Acts G &AllowedActs F = AllowedActs G)"
+by (blast intro: program_equalityI program_equalityE)
+
+
+(*** These rules allow "lazy" definition expansion 
+     They avoid expanding the full program, which is a large expression
+***)
+
+lemma def_prg_Init: "F == mk_program (init,acts,allowed) ==> Init F = init"
+by auto
+
+lemma def_prg_Acts:
+     "F == mk_program (init,acts,allowed) ==> Acts F = insert Id acts"
+by auto
+
+lemma def_prg_AllowedActs:
+     "F == mk_program (init,acts,allowed)  
+      ==> AllowedActs F = insert Id allowed"
+by auto
+
+(*The program is not expanded, but its Init and Acts are*)
+lemma def_prg_simps:
+    "[| F == mk_program (init,acts,allowed) |]  
+     ==> Init F = init & Acts F = insert Id acts"
+by simp
+
+(*An action is expanded only if a pair of states is being tested against it*)
+lemma def_act_simp:
+     "[| act == {(s,s'). P s s'} |] ==> ((s,s') : act) = P s s'"
+by auto
+
+(*A set is expanded only if an element is being tested against it*)
+lemma def_set_simp: "A == B ==> (x : A) = (x : B)"
+by auto
+
+
+(*** co ***)
+
+lemma constrainsI: 
+    "(!!act s s'. [| act: Acts F;  (s,s') : act;  s: A |] ==> s': A')  
+     ==> F : A co A'"
+by (simp add: constrains_def, blast)
+
+lemma constrainsD: 
+    "[| F : A co A'; act: Acts F;  (s,s'): act;  s: A |] ==> s': A'"
+by (unfold constrains_def, blast)
+
+lemma constrains_empty [iff]: "F : {} co B"
+by (unfold constrains_def, blast)
+
+lemma constrains_empty2 [iff]: "(F : A co {}) = (A={})"
+by (unfold constrains_def, blast)
+
+lemma constrains_UNIV [iff]: "(F : UNIV co B) = (B = UNIV)"
+by (unfold constrains_def, blast)
+
+lemma constrains_UNIV2 [iff]: "F : A co UNIV"
+by (unfold constrains_def, blast)
+
+(*monotonic in 2nd argument*)
+lemma constrains_weaken_R: 
+    "[| F : A co A'; A'<=B' |] ==> F : A co B'"
+by (unfold constrains_def, blast)
+
+(*anti-monotonic in 1st argument*)
+lemma constrains_weaken_L: 
+    "[| F : A co A'; B<=A |] ==> F : B co A'"
+by (unfold constrains_def, blast)
+
+lemma constrains_weaken: 
+   "[| F : A co A'; B<=A; A'<=B' |] ==> F : B co B'"
+by (unfold constrains_def, blast)
+
+(** Union **)
+
+lemma constrains_Un: 
+    "[| F : A co A'; F : B co B' |] ==> F : (A Un B) co (A' Un B')"
+by (unfold constrains_def, blast)
+
+lemma constrains_UN: 
+    "(!!i. i:I ==> F : (A i) co (A' i)) 
+     ==> F : (UN i:I. A i) co (UN i:I. A' i)"
+by (unfold constrains_def, blast)
+
+lemma constrains_Un_distrib: "(A Un B) co C = (A co C) Int (B co C)"
+by (unfold constrains_def, blast)
+
+lemma constrains_UN_distrib: "(UN i:I. A i) co B = (INT i:I. A i co B)"
+by (unfold constrains_def, blast)
+
+lemma constrains_Int_distrib: "C co (A Int B) = (C co A) Int (C co B)"
+by (unfold constrains_def, blast)
+
+lemma constrains_INT_distrib: "A co (INT i:I. B i) = (INT i:I. A co B i)"
+by (unfold constrains_def, blast)
+
+(** Intersection **)
+
+lemma constrains_Int: 
+    "[| F : A co A'; F : B co B' |] ==> F : (A Int B) co (A' Int B')"
+by (unfold constrains_def, blast)
+
+lemma constrains_INT: 
+    "(!!i. i:I ==> F : (A i) co (A' i)) 
+     ==> F : (INT i:I. A i) co (INT i:I. A' i)"
+by (unfold constrains_def, blast)
+
+lemma constrains_imp_subset: "F : A co A' ==> A <= A'"
+by (unfold constrains_def, auto)
+
+(*The reasoning is by subsets since "co" refers to single actions
+  only.  So this rule isn't that useful.*)
+lemma constrains_trans: 
+    "[| F : A co B; F : B co C |] ==> F : A co C"
+by (unfold constrains_def, blast)
+
+lemma constrains_cancel: 
+   "[| F : A co (A' Un B); F : B co B' |] ==> F : A co (A' Un B')"
+by (unfold constrains_def, clarify, blast)
+
+
+(*** unless ***)
+
+lemma unlessI: "F : (A-B) co (A Un B) ==> F : A unless B"
+by (unfold unless_def, assumption)
+
+lemma unlessD: "F : A unless B ==> F : (A-B) co (A Un B)"
+by (unfold unless_def, assumption)
+
+
+(*** stable ***)
+
+lemma stableI: "F : A co A ==> F : stable A"
+by (unfold stable_def, assumption)
+
+lemma stableD: "F : stable A ==> F : A co A"
+by (unfold stable_def, assumption)
+
+lemma stable_UNIV [simp]: "stable UNIV = UNIV"
+by (unfold stable_def constrains_def, auto)
+
+(** Union **)
+
+lemma stable_Un: 
+    "[| F : stable A; F : stable A' |] ==> F : stable (A Un A')"
+
+apply (unfold stable_def)
+apply (blast intro: constrains_Un)
+done
+
+lemma stable_UN: 
+    "(!!i. i:I ==> F : stable (A i)) ==> F : stable (UN i:I. A i)"
+apply (unfold stable_def)
+apply (blast intro: constrains_UN)
+done
+
+(** Intersection **)
+
+lemma stable_Int: 
+    "[| F : stable A;  F : stable A' |] ==> F : stable (A Int A')"
+apply (unfold stable_def)
+apply (blast intro: constrains_Int)
+done
+
+lemma stable_INT: 
+    "(!!i. i:I ==> F : stable (A i)) ==> F : stable (INT i:I. A i)"
+apply (unfold stable_def)
+apply (blast intro: constrains_INT)
+done
+
+lemma stable_constrains_Un: 
+    "[| F : stable C; F : A co (C Un A') |] ==> F : (C Un A) co (C Un A')"
+by (unfold stable_def constrains_def, blast)
+
+lemma stable_constrains_Int: 
+  "[| F : stable C; F :  (C Int A) co A' |] ==> F : (C Int A) co (C Int A')"
+by (unfold stable_def constrains_def, blast)
+
+(*[| F : stable C; F :  (C Int A) co A |] ==> F : stable (C Int A) *)
+lemmas stable_constrains_stable = stable_constrains_Int [THEN stableI, standard]
+
+
+(*** invariant ***)
+
+lemma invariantI: "[| Init F<=A;  F: stable A |] ==> F : invariant A"
+by (simp add: invariant_def)
+
+(*Could also say "invariant A Int invariant B <= invariant (A Int B)"*)
+lemma invariant_Int:
+     "[| F : invariant A;  F : invariant B |] ==> F : invariant (A Int B)"
+by (auto simp add: invariant_def stable_Int)
+
+
+(*** increasing ***)
+
+lemma increasingD: 
+     "F : increasing f ==> F : stable {s. z <= f s}"
+
+by (unfold increasing_def, blast)
+
+lemma increasing_constant [iff]: "F : increasing (%s. c)"
+by (unfold increasing_def stable_def, auto)
+
+lemma mono_increasing_o: 
+     "mono g ==> increasing f <= increasing (g o f)"
+apply (unfold increasing_def stable_def constrains_def, auto)
+apply (blast intro: monoD order_trans)
+done
+
+(*Holds by the theorem (Suc m <= n) = (m < n) *)
+lemma strict_increasingD: 
+     "!!z::nat. F : increasing f ==> F: stable {s. z < f s}"
+by (simp add: increasing_def Suc_le_eq [symmetric])
+
+
+(** The Elimination Theorem.  The "free" m has become universally quantified!
+    Should the premise be !!m instead of ALL m ?  Would make it harder to use
+    in forward proof. **)
+
+lemma elimination: 
+    "[| ALL m:M. F : {s. s x = m} co (B m) |]  
+     ==> F : {s. s x : M} co (UN m:M. B m)"
+by (unfold constrains_def, blast)
+
+(*As above, but for the trivial case of a one-variable state, in which the
+  state is identified with its one variable.*)
+lemma elimination_sing: 
+    "(ALL m:M. F : {m} co (B m)) ==> F : M co (UN m:M. B m)"
+by (unfold constrains_def, blast)
+
+
+
+(*** Theoretical Results from Section 6 ***)
+
+lemma constrains_strongest_rhs: 
+    "F : A co (strongest_rhs F A )"
+by (unfold constrains_def strongest_rhs_def, blast)
+
+lemma strongest_rhs_is_strongest: 
+    "F : A co B ==> strongest_rhs F A <= B"
+by (unfold constrains_def strongest_rhs_def, blast)
+
+
+(** Ad-hoc set-theory rules **)
+
+lemma Un_Diff_Diff [simp]: "A Un B - (A - B) = B"
+by blast
+
+lemma Int_Union_Union: "Union(B) Int A = Union((%C. C Int A)`B)"
+by blast
+
+(** Needed for WF reasoning in WFair.ML **)
+
+lemma Image_less_than [simp]: "less_than `` {k} = greaterThan k"
+by blast
+
+lemma Image_inverse_less_than [simp]: "less_than^-1 `` {k} = lessThan k"
+by blast
 
 end
